Add interp-correctness condition for rewriter
The NBE-rewrite rules are proven correct.  The arith and fancy rewrite
rules are reduced to lemmas about Z, most of which are inconsistent (and
therefore indicate rewrite rules which are missing side-conditions).

One bad rewrite rule was found in this process, and corrected in
0842563b23f8d780f4ff1080d7620fc3f368191f

The next step after this will be using the rewrite rule correctness to
prove the rewriter correct.

src/Experiments/NewPipeline/RewriterWf1.v
@@ -204,6 +204,9 @@ Module Compilers.
 
                 (full_types : raw_pident -> Type)
                 (invert_bind_args invert_bind_args_unknown : forall t (idc : ident t) (pidc : raw_pident), option (full_types pidc))
+                (pident_to_typed
+                 : forall t (idc : pident t) (evm : EvarMap),
+                    type_of_list (pident_arg_types t idc) -> ident (pattern.type.subst_default t evm))
                 (type_of_raw_pident : forall (pidc : raw_pident), full_types pidc -> type.type base.type)
                 (raw_pident_to_typed : forall (pidc : raw_pident) (args : full_types pidc), ident (type_of_raw_pident pidc args))
                 (raw_pident_is_simple : raw_pident -> bool)
@@ -236,15 +239,24 @@ Module Compilers.
         Local Notation to_raw_pattern := (@pattern.to_raw pident raw_pident (@strip_types)).
         Local Notation reify := (@reify ident).
         Local Notation reflect := (@reflect ident).
+        Local Notation reify_expr := (@reify_expr ident).
         Local Notation rawexpr := (@rawexpr ident).
         Local Notation eval_decision_tree var := (@eval_decision_tree ident var pident full_types invert_bind_args type_of_raw_pident raw_pident_to_typed).
         Local Notation reveal_rawexpr e := (@reveal_rawexpr_cps ident _ e _ id).
         Local Notation unify_pattern' var := (@unify_pattern' ident var pident pident_arg_types pident_unify pident_unify_unknown).
         Local Notation unify_pattern var := (@unify_pattern ident var pident pident_arg_types pident_unify pident_unify_unknown type_vars_of_pident).
 
+        Definition lam_type_of_list {ls K} : (type_of_list ls -> K) -> type_of_list_cps K ls
+          := list_rect
+               (fun ls => (type_of_list ls -> K) -> type_of_list_cps K ls)
+               (fun f => f tt)
+               (fun T Ts rec k t => rec (fun ts => k (t, ts)))
+               ls.
+
         Section with_var1.
           Context {var : type -> Type}.
           Local Notation expr := (@expr.expr base.type ident var).
+          Local Notation deep_rewrite_ruleTP_gen := (@deep_rewrite_ruleTP_gen ident var).
 
           Local Notation "e1 === e2" := (existT expr _ e1 = existT expr _ e2) : type_scope.
 
@@ -572,27 +584,37 @@ Module Compilers.
                          | break_match_step ltac:(fun _ => idtac) ].
           Qed.
 
-          Lemma normalize_deep_rewrite_rule_cps_id
-                {should_do_again with_opt under_lets is_cps t v T k}
-                (Hk : k None = None)
-                (Hv : (match is_cps, with_opt return @deep_rewrite_ruleTP_gen ident var should_do_again with_opt under_lets is_cps t -> Prop
-                       with
-                       | true, true => fun v => forall T k, v T k = k (v _ id)
-                       | true, false => fun v => forall T k, v T k = (v' <- v _ (@Some _); k v')%option
-                       | false, _ => fun _ => True
-                       end)
-                        v)
-            : @normalize_deep_rewrite_rule ident var should_do_again with_opt under_lets is_cps t v T k = k (@normalize_deep_rewrite_rule ident var should_do_again with_opt under_lets is_cps t v _ id).
-          Proof using Type.
-            clear -Hv Hk; cbn in *.
-            repeat first [ progress cbn in *
-                         | progress destruct_head'_bool
-                         | reflexivity
-                         | progress cbv [id Option.bind] in *
-                         | solve [ auto ]
-                         | break_innermost_match_step
-                         | rewrite Hv; (solve [ auto ] + break_innermost_match_step) ].
-          Qed.
+          Section normalize_deep_rewrite_rule_cps_id.
+            Context {should_do_again with_opt under_lets is_cps : bool}
+                    {t}
+                    {v : @deep_rewrite_ruleTP_gen should_do_again with_opt under_lets is_cps t}
+                    {T}
+                    {k : option (UnderLets var (@expr.expr base.type ident (if should_do_again then @value var else var) t)) -> option T}.
+
+            Definition normalize_deep_rewrite_rule_cps_id_hypsT
+              := ((match is_cps, with_opt return @deep_rewrite_ruleTP_gen should_do_again with_opt under_lets is_cps t -> Prop
+                   with
+                   | true, true => fun v => forall T k, v T k = k (v _ id)
+                   | true, false => fun v => forall T k, v T k = (v' <- v _ (@Some _); k v')%option
+                   | false, _ => fun _ => True
+                   end)
+                    v).
+
+            Lemma normalize_deep_rewrite_rule_cps_id
+                  (Hk : k None = None)
+                  (Hv : normalize_deep_rewrite_rule_cps_id_hypsT)
+              : @normalize_deep_rewrite_rule ident var should_do_again with_opt under_lets is_cps t v T k = k (@normalize_deep_rewrite_rule ident var should_do_again with_opt under_lets is_cps t v _ id).
+            Proof using Type.
+              clear -Hk Hv; cbv [normalize_deep_rewrite_rule_cps_id_hypsT] in *; cbn in *.
+              repeat first [ progress cbn in *
+                           | progress destruct_head'_bool
+                           | reflexivity
+                           | progress cbv [id Option.bind] in *
+                           | solve [ auto ]
+                           | break_innermost_match_step
+                           | rewrite Hv; (solve [ auto ] + break_innermost_match_step) ].
+            Qed.
+          End normalize_deep_rewrite_rule_cps_id.
         End with_var1.
 
         Section with_var2.
@@ -669,6 +691,26 @@ Module Compilers.
               eapply He; rewrite app_assoc; wf_t. }
             { eapply He with (seg:=nil); [ reflexivity | ].
               eapply wf_reify; auto. }
+          Qed.
+
+          Lemma wf_reify_expr G G' {t}
+                (HG : forall t v1 v2, List.In (existT _ t (v1, v2)) G -> @wf_value G' t v1 v2)
+                e1 e2
+                (Hwf : expr.wf G e1 e2)
+            : expr.wf G' (@reify_expr var1 t e1) (@reify_expr var2 t e2).
+          Proof using Type.
+            cbv [wf_value] in *; revert dependent G'; induction Hwf; intros; cbn [reify_expr];
+              first [ constructor | apply wf_reify ]; eauto; intros.
+            all: match goal with H : _ |- _ => apply H end.
+            all: repeat first [ progress cbn [In eq_rect] in *
+                              | progress intros
+                              | progress destruct_head'_or
+                              | progress subst
+                              | progress inversion_sigma
+                              | progress inversion_prod
+                              | apply wf_reflect
+                              | solve [ eapply wf_value'_Proper_list; [ | solve [ eauto ] ]; wf_safe_t ]
+                              | constructor ].
           Qed.
 
           Inductive wf_rawexpr : list { t : type & var1 t * var2 t }%type -> forall {t}, @rawexpr var1 -> @expr var1 t -> @rawexpr var2 -> @expr var2 t -> Prop :=
@@ -994,6 +1036,137 @@ Module Compilers.
                                (rew [fun tp => @rewrite_rule_data1 _ (pattern.pattern_of_anypattern tp)] pf in r1)
                                r2 }).
         End with_var2.
+
+        Section with_interp.
+          Context (ident_interp : forall t, ident t -> type.interp base.interp t)
+                  {ident_interp_Proper : forall t, Proper (eq ==> type.eqv) (ident_interp t)}.
+          Local Notation var := (type.interp base.interp) (only parsing).
+          Local Notation expr := (@expr.expr base.type ident var).
+          Local Notation rewrite_rulesT := (@rewrite_rulesT ident var pident pident_arg_types type_vars_of_pident).
+          Local Notation rewrite_rule_data := (@rewrite_rule_data ident var pident pident_arg_types type_vars_of_pident).
+          Local Notation with_unif_rewrite_ruleTP_gen := (@with_unif_rewrite_ruleTP_gen ident var pident pident_arg_types type_vars_of_pident).
+          Local Notation with_unification_resultT' := (@with_unification_resultT' ident var pident pident_arg_types).
+          Local Notation normalize_deep_rewrite_rule := (@normalize_deep_rewrite_rule ident var).
+          Local Notation under_with_unification_resultT_relation := (@under_with_unification_resultT_relation ident var pident pident_arg_types type_vars_of_pident).
+          Local Notation under_with_unification_resultT_relation_hetero := (@under_with_unification_resultT_relation_hetero ident var pident pident_arg_types type_vars_of_pident).
+          Local Notation deep_rewrite_ruleTP_gen := (@deep_rewrite_ruleTP_gen ident var).
+
+          Local Notation UnderLets_maybe_interp with_lets
+            := (if with_lets as with_lets' return (if with_lets' then UnderLets var _ else _) -> _
+                then UnderLets.interp ident_interp
+                else (fun x => x)).
+
+          Fixpoint value'_interp_related
+                   {with_lets1 with_lets2 t}
+            : @value' var with_lets1 t
+              -> @value' var with_lets2 t
+              -> Prop
+            := match t return value' _ t -> value' _ t -> Prop with
+               | type.base t
+                 => fun v1 v2
+                    => expr.interp ident_interp (UnderLets_maybe_interp with_lets1 v1)
+                       == expr.interp ident_interp (UnderLets_maybe_interp with_lets2 v2)
+               | type.arrow s d
+                 => fun (f1 f2 : value' _ s -> value' _ d)
+                    => forall x1 x2,
+                        @value'_interp_related _ _ s x1 x2
+                        -> @value'_interp_related _ _ d (f1 x1) (f2 x2)
+               end.
+
+          Definition value_interp_related {t} : relation (@value var t)
+            := value'_interp_related.
+
+          Lemma interp_reify_reflect {with_lets t} e v
+            : expr.interp ident_interp e == v -> expr.interp ident_interp (@reify _ with_lets t (reflect e)) == v.
+          Proof using Type.
+            revert with_lets; induction t as [|s IHs d IHd]; intro;
+              cbn [type.related reflect reify];
+              fold (@reify var) (@reflect var); cbv [respectful]; break_innermost_match;
+                cbn [expr.interp UnderLets.to_expr]; auto; [].
+            intros Hf ? ? Hx.
+            apply IHd; cbn [expr.interp]; auto.
+          Qed.
+
+          Lemma interp_of_wf_reify_expr G {t}
+                (HG : forall t v1 v2, List.In (existT _ t (v1, v2)) G -> expr.interp ident_interp (reify v1) == v2)
+                e1 e2
+                (Hwf : expr.wf G e1 e2)
+            : expr.interp ident_interp (@reify_expr _ t e1) == expr.interp ident_interp e2.
+          Proof using ident_interp_Proper.
+            induction Hwf; cbn [expr.interp reify_expr]; cbv [LetIn.Let_In];
+              try solve [ auto
+                        | apply ident_interp_Proper; reflexivity ].
+            all: cbn [type.related] in *; cbv [respectful]; intros.
+            all: match goal with H : _ |- _ => apply H; clear H end.
+            all: repeat first [ progress cbn [In eq_rect fst snd] in *
+                              | progress intros
+                              | progress destruct_head'_or
+                              | progress subst
+                              | progress inversion_sigma
+                              | progress inversion_prod
+                              | apply interp_reify_reflect
+                              | solve [ auto ] ].
+          Qed.
+
+          Fixpoint pattern_default_interp' {K t} (p : pattern t) evm {struct p} : (expr (pattern.type.subst_default t evm) -> K) -> @with_unification_resultT' t p evm K
+            := match p in pattern.pattern t return (expr (pattern.type.subst_default t evm) -> K) -> @with_unification_resultT' t p evm K with
+               | pattern.Wildcard t => fun k v => k (reify v)
+               | pattern.Ident t idc
+                 => fun k
+                    => lam_type_of_list (fun args => k (expr.Ident (pident_to_typed _ idc _ args)))
+               | pattern.App s d f x
+                 => fun k
+                    => @pattern_default_interp'
+                         _ _ f evm
+                         (fun ef
+                          => @pattern_default_interp'
+                               _ _ x evm
+                               (fun ex
+                                => k (expr.App ef ex)))
+               end.
+
+          Definition pattern_default_interp {t} (p : pattern t) : @with_unif_rewrite_ruleTP_gen t p false false false false
+            := pattern.type.lam_forall_vars
+                 (fun evm
+                  => pattern_default_interp' p evm id).
+
+          Definition deep_rewrite_ruleTP_gen_good_relation
+                     {should_do_again with_opt under_lets is_cps : bool} {t}
+                     (v1 : @deep_rewrite_ruleTP_gen should_do_again with_opt under_lets is_cps t)
+                     (v2 : expr t)
+            : Prop
+            := @normalize_deep_rewrite_rule_cps_id_hypsT var _ _ _ _ _ v1
+               /\ (let v1 := normalize_deep_rewrite_rule v1 _ id in
+                   match v1 with
+                   | None => True
+                   | Some v1 => let v1 := UnderLets.interp ident_interp v1 in
+                                (if should_do_again
+                                    return (@expr.expr base.type ident (if should_do_again then @value var else var) t) -> Prop
+                                 then
+                                   (fun v1
+                                    => expr.interp ident_interp (reify_expr v1) == expr.interp ident_interp v2)
+                                 else
+                                   (fun v1 => expr.interp ident_interp v1 == expr.interp ident_interp v2))
+                                  v1
+                   end).
+
+          Definition rewrite_rule_data_interp_goodT
+                     {t} {p : pattern t} (r : @rewrite_rule_data t p)
+            : Prop
+            := @under_with_unification_resultT_relation_hetero
+                 _ _ _ _
+                 (fun _ => value_interp_related)
+                 (fun evm => deep_rewrite_ruleTP_gen_good_relation)
+                 (rew_replacement _ _ r)
+                 (pattern_default_interp p).
+
+          Definition rewrite_rules_interp_goodT
+                     (rews : rewrite_rulesT)
+            : Prop
+            := forall p r,
+              List.In (existT _ p r) rews
+              -> rewrite_rule_data_interp_goodT r.
+        End with_interp.
       End with_var.
     End Compile.
   End RewriteRules.
